---
tags: [discrete-structures, prelims, logic, propositional-logic, applications]
---
# Applications of Propositional Logic

> [!summary] What this covers
> Translating English to logic, system specifications, propositional equivalences (tautologies, contradictions, De Morgan's Laws), and satisfiability.

## Contents

- [[#Translating English Sentences]]
- [[#System Specifications]]
- [[#Propositional Equivalences]]
- [[#De Morgan's Laws]]
- [[#Logical Equivalences]]
- [[#Equivalence Proofs]]
- [[#Propositional Satisfiability]]

---

## Translating English Sentences

Converting English to propositional logic:
1. Identify atomic propositions â†’ assign variables
2. Determine the logical connectives

> [!example] Translation Example
> "If I go to Harry's or to the country, I will not go shopping."
> 
> Variables:
> - $p$: I go to Harry's
> - $q$: I go to the country
> - $r$: I will go shopping
> 
> **Logic:** $(p \lor q) \to \neg r$

> [!example] "Only if" Translation
> "You can access the Internet from campus **only if** you are a computer science major **or** you are **not** a freshman."
> 
> Variables:
> - $a$: You can access the internet from campus
> - $c$: You are a computer science major
> - $f$: You are a freshman
> 
> **Logic:** $a \to (c \lor \neg f)$

---

## System Specifications

Engineers take requirements in English and express them precisely using logic.

> [!example] System Spec Example
> "The automated reply cannot be sent when the file system is full."
> 
> - $x$: The automated reply can be sent
> - $y$: The file system is full
> 
> **Logic:** $y \to \neg x$

---

## Propositional Equivalences

> [!info]+ ðŸ“Š Tautology vs Contradiction
> ![[attachments/tautology_contradiction.png]]
> *A tautology is always true; a contradiction is always false*

> [!definition] Terms
> **Tautology** â€” a proposition that's always true (e.g., $p \lor \neg p$)
> 
> **Contradiction** â€” a proposition that's always false (e.g., $p \land \neg p$)
> 
> **Contingency** â€” neither tautology nor contradiction (depends on values)

| $p$ | $\neg p$ | $p \lor \neg p$ | $p \land \neg p$ |
| :-: | :------: | :-------------: | :--------------: |
|  T  |    F     |        T        |        F         |
|  F  |    T     |        T        |        F         |

### Logical Equivalence

Two propositions $p$ and $q$ are **logically equivalent** if $p \leftrightarrow q$ is a tautology.

We write: $p \equiv q$ or $p \Leftrightarrow q$

They're equivalent if their truth table columns match.

> [!example] Equivalence Example
> $\neg p \lor q$ is equivalent to $p \to q$:
> 
> | $p$ | $q$ | $\neg p$ | $\neg p \lor q$ | $p \to q$ |
> |:---:|:---:|:---:|:---:|:---:|
> | T | T | F | T | T |
> | T | F | F | F | F |
> | F | T | T | T | T |
> | F | F | T | T | T |

---
## De Morgan's Laws

Named after Augustus De Morgan (1806-1871).

> [!info]+ ðŸ“Š De Morgan's Laws
> ![[attachments/demorgan_laws.png]]
> *NOT distributes and flips the operator*
> Negation distributes and flips ANDâ†”OR.

| $p$ | $q$ | $\neg p$ | $\neg q$ | $p \lor q$ | $\neg(p \lor q)$ | $\neg p \land \neg q$ |
|:---:|:---:|:---:|:---:|:---:|:---:|:---:|
| T | T | F | F | T | F | F |
| T | F | F | T | T | F | F |
| F | T | T | F | T | F | F |
| F | F | T | T | F | T | T |

---

## Logical Equivalences

> [!abstract] Fundamental Laws
> | Law | Equivalence |
> |---|---|
> | **Identity** | $p \land T \equiv p$, $p \lor F \equiv p$ |
> | **Domination** | $p \lor T \equiv T$, $p \land F \equiv F$ |
> | **Idempotent** | $p \lor p \equiv p$, $p \land p \equiv p$ |
> | **Double Negation** | $\neg(\neg p) \equiv p$ |
> | **Negation** | $p \lor \neg p \equiv T$, $p \land \neg p \equiv F$ |
> | **Commutative** | $p \lor q \equiv q \lor p$, $p \land q \equiv q \land p$ |
> | **Associative** | $(p \lor q) \lor r \equiv p \lor (q \lor r)$ |
> | **Distributive** | $p \lor (q \land r) \equiv (p \lor q) \land (p \lor r)$ |
> | **Absorption** | $p \lor (p \land q) \equiv p$, $p \land (p \lor q) \equiv p$ |

### Conditional Equivalences

> [!info] Involving $\to$
> - $p \to q \equiv \neg p \lor q$
> - $p \to q \equiv \neg q \to \neg p$ (contrapositive)
> - $\neg(p \to q) \equiv p \land \neg q$

### Biconditional Equivalences

> [!info] Involving $\leftrightarrow$
> - $p \leftrightarrow q \equiv (p \to q) \land (q \to p)$
> - $p \leftrightarrow q \equiv (p \land q) \lor (\neg p \land \neg q)$

---

## Equivalence Proofs

To prove $A \equiv B$, chain equivalences: $A \equiv A_1 \equiv \ldots \equiv B$

> [!example] Proof 1
> **Show:** $\neg(p \lor (\neg p \land q)) \equiv \neg p \land \neg q$
> 
> $$\begin{aligned}
> \neg(p \lor (\neg p \land q)) &\equiv \neg p \land \neg(\neg p \land q) & \text{(De Morgan)} \\
> &\equiv \neg p \land (p \lor \neg q) & \text{(De Morgan + Double Neg)} \\
> &\equiv (\neg p \land p) \lor (\neg p \land \neg q) & \text{(Distributive)} \\
> &\equiv F \lor (\neg p \land \neg q) & \text{(Negation law)} \\
> &\equiv \neg p \land \neg q & \text{(Identity)}
> \end{aligned}$$

> [!example] Proof 2 â€” Tautology
> **Show:** $(p \land q) \to (p \lor q)$ is a tautology
> 
> $$\begin{aligned}
> (p \land q) \to (p \lor q) &\equiv \neg(p \land q) \lor (p \lor q) \\
> &\equiv (\neg p \lor \neg q) \lor (p \lor q) & \text{(De Morgan)} \\
> &\equiv (\neg p \lor p) \lor (\neg q \lor q) & \text{(Rearrange)} \\
> &\equiv T \lor T \equiv T
> \end{aligned}$$

---
## Propositional Satisfiability

> [!definition] Satisfiability
> A compound proposition is **satisfiable** if some assignment of truth values makes it true.
> 
> If no assignment works, it's **unsatisfiable** (and its negation is a tautology).

> [!example] Satisfiability Examples
> **1.** $(p \lor \neg q) \land (q \lor \neg r) \land (r \lor \neg p)$
> âœ… Satisfiable â€” set $p, q, r$ all to T
> 
> **2.** $(p \lor q \lor r) \land (\neg p \lor \neg q \lor \neg r)$
> âœ… Satisfiable â€” set $p = T$, $q = F$
> 
> **3.** Combining 1 and 2:
> âŒ Not satisfiable â€” no assignment works

---
## Notation
> [!info] Shorthand
> $\bigvee_{j=1}^{n} p_j$ is used for $p_1 \lor p_2 \lor \ldots \lor p_n$
> 
> $\bigwedge_{j=1}^{n} p_j$ is used for $p_1 \land p_2 \land \ldots \land p_n$


>[!example] Exercise Answers
> **Prove:** $\neg (p \neg q) \lor (\neg p \land q) \equiv (\neg p \land \neg (\neg q)) \lor (\neg p \land \neg q)$ 
> $$\equiv (\neg p \land \neg (\neg q)) \lor (\neg p \land \neg q) \rightarrow De \ Morgan's \ Law$$
> $$\equiv (\neg p \land q) \lor (\neg p \land \neg q) \rightarrow Double \ Negation$$
> $$\equiv \neg p \land (q \lor \neg q) \rightarrow Distributive$$
> $$\equiv \neg p \land T \rightarrow Negation$$
> $$\equiv \neg p \rightarrow Identity$$ 
