---
tags: [discrete-structures, prelims, logic, inference, arguments, proofs]
---
# Rules of Inference

> [!summary] What this covers
> Valid arguments, rules of inference for propositional logic (Modus Ponens, Modus Tollens, etc.), rules of inference for quantified statements (UI, UG, EI, EG), and constructing valid arguments.

## Contents

- [[#Arguments and Validity]]
- [[#Rules of Inference for Propositional Logic]]
- [[#Building Valid Arguments]]
- [[#Rules of Inference for Quantified Statements]]
- [[#Quantified Argument Examples]]

---

## Arguments and Validity

Recall the Socrates example from predicate logic:
- "All men are mortal."
- "Socrates is a man."
- Therefore: "Socrates is mortal."

We intuitively know this conclusion follows from the premises. But how do we *formally* justify it? That's what rules of inference are for. They give us a rigorous way to derive conclusions from premises.

This can be expressed as an argument with premises above the line and conclusion below:

$$\frac{\forall x(Man(x) \to Mortal(x)) \\ Man(Socrates)}{\therefore Mortal(Socrates)}$$

> [!definition] Argument
> A sequence of propositions where all but the final one are **premises** and the last is the **conclusion**.
> 
> An argument is **valid** if the premises imply the conclusion.

> [!info] Validity as Tautology
> If premises are $p_1, p_2, \ldots, p_n$ and conclusion is $q$, then the argument is valid if:
> $$(p_1 \land p_2 \land \ldots \land p_n) \to q$$
> is a tautology.
> 
> So basically, "if all premises are true, the conclusion *must* be true."

We construct valid arguments in two stages:
1. **Propositional Logic:** Basic inference rules
2. **Predicate Logic:** Propositional rules + rules for quantifiers

---

## Rules of Inference for Propositional Logic

These are the building blocks for constructing valid arguments. Each rule is a simple, proven argument form that we can apply whenever the pattern matches.

> [!info]+ ðŸ“Š Rules Overview
> ![[attachments/inference_rules.png]]
> *Propositional rules on left, quantifier rules on right*

### Modus Ponens

The most common and intuitive rule. "If P then Q. P is true. So Q must be true."

$$\frac{p \to q \\ p}{\therefore q}$$

> [!info] Corresponding Tautology
> $(p \land (p \to q)) \to q$

> [!example] Modus Ponens
> - $p$: "It is snowing."
> - $q$: "I will study discrete math."
> 
> "If it is snowing, then I will study discrete math."
> "It is snowing."
> **Therefore:** "I will study discrete math."
> 
> The condition was met, so the consequence follows. Simple as that.

---

### Modus Tollens

The "contrapositive reasoning" rule. If P implies Q, and Q is false, then P must have been false too. Otherwise, P being true would have made Q true (contradiction).

$$\frac{p \to q \\ \neg q}{\therefore \neg p}$$

> [!info] Corresponding Tautology
> $(\neg q \land (p \to q)) \to \neg p$

> [!example] Modus Tollens
> - $p$: "It is snowing."
> - $q$: "I will study discrete math."
> 
> "If it is snowing, then I will study discrete math."
> "I will not study discrete math."
> **Therefore:** "It is not snowing."
> 
> The consequence didn't happen, so the condition couldn't have been true. Reasoning backwards.

---

### Hypothetical Syllogism

Chaining implications together. If A leads to B, and B leads to C, then A leads to C. Lets you skip the middle step.

$$\frac{p \to q \\ q \to r}{\therefore p \to r}$$

> [!info] Corresponding Tautology
> $((p \to q) \land (q \to r)) \to (p \to r)$

> [!example] Hypothetical Syllogism
> - $p$: "It snows."
> - $q$: "I will study discrete math."
> - $r$: "I will get an A."
> 
> "If it snows, then I will study discrete math."
> "If I study discrete math, I will get an A."
> **Therefore:** "If it snows, I will get an A."
> 
> Chained the implications together. The middle step ($q$) served as a bridge.

### Disjunctive Syllogism

Process of elimination. If it's one or the other, and it's not this one, then it must be that one.

$$\frac{p \lor q \\ \neg p}{\therefore q}$$

> [!info] Corresponding Tautology
> $(\neg p \land (p \lor q)) \to q$

> [!example] Disjunctive Syllogism
> - $p$: "I will study discrete math."
> - $q$: "I will study English literature."
> 
> "I will study discrete math or I will study English literature."
> "I will not study discrete math."
> **Therefore:** "I will study English literature."
> 
> One option was eliminated, so the other must be true.

### Addition

$$\frac{p}{\therefore p \lor q}$$

> [!info] Corresponding Tautology
> $p \to (p \lor q)$

If something is true, you can OR it with *anything* and it's still true. Seems almost too easy, but it's useful when you need to introduce a new proposition into an argument.

> [!example] Addition
> - $p$: "I will study discrete math."
> - $q$: "I will visit Las Vegas."
> 
> "I will study discrete math."
> **Therefore:** "I will study discrete math or I will visit Las Vegas."
> 
> We didn't prove anything about Las Vegas, but the OR statement is still true because the first part is.

### Simplification

$$\frac{p \land q}{\therefore p}$$

> [!info] Corresponding Tautology
> $(p \land q) \to p$

If a conjunction is true, then each part must be true. You can "extract" either side from an AND.

> [!example] Simplification
> - $p$: "I will study discrete math."
> - $q$: "I will study English literature."
> 
> "I will study discrete math and English literature."
> **Therefore:** "I will study discrete math."
> 
> If you committed to both, you definitely committed to each one individually.

### Conjunction

$$\frac{p \\ q}{\therefore p \land q}$$

> [!info] Corresponding Tautology
> $((p) \land (q)) \to (p \land q)$

If two things are separately true, you can combine them with AND. The reverse of simplification.

> [!example] Conjunction
> - $p$: "I will study discrete math."
> - $q$: "I will study English literature."
> 
> "I will study discrete math."
> "I will study English literature."
> **Therefore:** "I will study discrete math and I will study English literature."
> 
> Two separate facts combine into one.

### Resolution

$$\frac{\neg p \lor r \\ p \lor q}{\therefore q \lor r}$$

> [!info] Corresponding Tautology
> $((\neg p \lor r) \land (p \lor q)) \to (q \lor r)$

This one's trickier. The idea: $p$ and $\neg p$ "cancel out" because one of them must be false. Whatever's left on each side ($q$ and $r$) gets ORed together.

> [!example] Resolution
> - $p$: "I will study discrete math."
> - $q$: "I will study databases."
> - $r$: "I will study English literature."
> 
> "I will not study discrete math or I will study English literature."
> "I will study discrete math or I will study databases."
> **Therefore:** "I will study databases or I will study English literature."
> 
> Either $p$ is true or it isn't. If it is, then $r$ follows from the first statement. If it isn't, then $q$ follows from the second. Either way, we get $q \lor r$.

> [!tip] Application
> Resolution plays an important role in AI and is used in Prolog. It's the basis for automated theorem proving.

---

## Summary Table

> [!abstract] Rules of Inference Reference
> | Rule | Form | What it means |
> |---|---|---|
> | Modus Ponens | $p \to q, p \Rightarrow q$ | Condition met, consequence follows |
> | Modus Tollens | $p \to q, \neg q \Rightarrow \neg p$ | Consequence failed, condition was false |
> | Hypothetical Syllogism | $p \to q, q \to r \Rightarrow p \to r$ | Chain implications together |
> | Disjunctive Syllogism | $p \lor q, \neg p \Rightarrow q$ | Process of elimination |
> | Addition | $p \Rightarrow p \lor q$ | Add anything via OR |
> | Simplification | $p \land q \Rightarrow p$ | Extract from AND |
> | Conjunction | $p, q \Rightarrow p \land q$ | Combine via AND |
> | Resolution | $\neg p \lor r, p \lor q \Rightarrow q \lor r$ | Cancel out $p$ and $\neg p$ |

---

## Building Valid Arguments

A valid argument is a sequence of statements where each is either:
- A premise, OR
- Follows from previous statements by rules of inference

The last statement is the conclusion. Each step must be justified by citing which rule and which previous steps you used.

> [!example] Example 1: Simple Argument
> From $p \land (p \to q)$, show that $q$ is a conclusion.
> 
> | Step | Reason |
> |---|---|
> | 1. $p \land (p \to q)$ | Premise |
> | 2. $p$ | Simplification using (1) |
> | 3. $p \to q$ | Simplification using (1) |
> | 4. $q$ | Modus Ponens using (2) and (3) |
> 
> We break apart the conjunction, then apply Modus Ponens to get the result.

> [!example] Example 2: Weather and Activities
> **Hypotheses:**
> - "It is not sunny this afternoon and it is colder than yesterday."
> - "We will go swimming only if it is sunny."
> - "If we do not go swimming, then we will take a canoe trip."
> - "If we take a canoe trip, then we will be home by sunset."
> 
> **Conclusion:** "We will be home by sunset."
> 
> **Variables:**
> - $p$: "It is sunny this afternoon."
> - $q$: "It is colder than yesterday."
> - $r$: "We will go swimming."
> - $s$: "We will take a canoe trip."
> - $t$: "We will be home by sunset."
> 
> **Translation:** $\neg p \land q$, $r \to p$, $\neg r \to s$, $s \to t$
> 
> | Step | Reason |
> |---|---|
> | 1. $\neg p \land q$ | Premise |
> | 2. $\neg p$ | Simplification using (1) |
> | 3. $r \to p$ | Premise |
> | 4. $\neg r$ | Modus Tollens using (2) and (3) |
> | 5. $\neg r \to s$ | Premise |
> | 6. $s$ | Modus Ponens using (4) and (5) |
> | 7. $s \to t$ | Premise |
> | 8. $t$ | Modus Ponens using (6) and (7) |
> 
> The main insight: we use Modus Tollens at step 4. Since $r \to p$ and $\neg p$, we conclude $\neg r$. Then we chain forward with Modus Ponens.

---

## Rules of Inference for Quantified Statements

For quantified statements, we need additional rules beyond propositional logic. These let us move between "for all" / "there exists" statements and specific instances.

### Universal Instantiation (UI)

$$\frac{\forall x\, P(x)}{\therefore P(c)}$$

If something holds for *all* $x$, it certainly holds for any specific $c$ we pick. This is how we go from general statements to specific ones.

> [!example] UI Example
> Domain: all dogs. Fido is a dog.
> 
> "All dogs are cuddly."
> **Therefore:** "Fido is cuddly."

---

### Universal Generalization (UG)

$$\frac{P(c) \text{ for an arbitrary } c}{\therefore \forall x\, P(x)}$$

If something holds for an *arbitrary* element (not a specific one we chose for special properties), then it holds for all elements.

> [!warning] Be careful
> The element $c$ must be truly arbitrary, not specially chosen. This is used often implicitly in mathematical proofs when we say "let $x$ be any element..."

---

### Existential Instantiation (EI)

$$\frac{\exists x\, P(x)}{\therefore P(c) \text{ for some element } c}$$

If we know something exists with a property, we can give it a name and work with it. We just can't assume anything else about it besides what we know.

> [!example] EI Example
> "There is someone who got an A in the course."
> **Therefore:** "Let's call her $a$ and say that $a$ got an A."

---

### Existential Generalization (EG)

$$\frac{P(c) \text{ for some element } c}{\therefore \exists x\, P(x)}$$

If a specific element has a property, then *something* has that property. We can go from specific to existential.

> [!example] EG Example
> "Michelle got an A in the class."
> **Therefore:** "Someone got an A in the class."

---

## Quantifier Rules Summary

> [!abstract] Quantifier Inference Rules
> | Rule | Form | Direction |
> |---|---|---|
> | Universal Instantiation (UI) | $\forall x\, P(x) \Rightarrow P(c)$ | General â†’ Specific |
> | Universal Generalization (UG) | $P(c)$ arbitrary $\Rightarrow \forall x\, P(x)$ | Specific â†’ General |
> | Existential Instantiation (EI) | $\exists x\, P(x) \Rightarrow P(c)$ for some $c$ | Name the witness |
> | Existential Generalization (EG) | $P(c) \Rightarrow \exists x\, P(x)$ | Specific â†’ Exists |

The pattern: UI and EI go from quantified to specific. UG and EG go from specific to quantified.

---

## Quantified Argument Examples

> [!example] Example 1: John Smith Has Two Legs
> **Premises:**
> - "Every man has two legs."
> - "John Smith is a man."
> 
> **Conclusion:** "John Smith has two legs."
> 
> Let $M(x)$ = "$x$ is a man", $L(x)$ = "$x$ has two legs", $J$ = John Smith.
> 
> | Step | Reason |
> |---|---|
> | 1. $\forall x(M(x) \to L(x))$ | Premise |
> | 2. $M(J) \to L(J)$ | UI from (1) |
> | 3. $M(J)$ | Premise |
> | 4. $L(J)$ | Modus Ponens using (2) and (3) |
> 
> We use UI to instantiate the universal statement for John specifically, then apply Modus Ponens.

> [!example] Example 2: Class and Book
> **Premises:**
> - "A student in this class has not read the book."
> - "Everyone in this class passed the first exam."
> 
> **Conclusion:** "Someone who passed the first exam has not read the book."
> 
> Let $C(x)$ = "$x$ is in this class", $B(x)$ = "$x$ has read the book", $P(x)$ = "$x$ passed the first exam."
> 
> $$\frac{\exists x(C(x) \land \neg B(x)) \\ \forall x(C(x) \to P(x))}{\therefore \exists x(P(x) \land \neg B(x))}$$
> 
> | Step | Reason |
> |---|---|
> | 1. $\exists x(C(x) \land \neg B(x))$ | Premise |
> | 2. $C(a) \land \neg B(a)$ | EI from (1) |
> | 3. $C(a)$ | Simplification from (2) |
> | 4. $\forall x(C(x) \to P(x))$ | Premise |
> | 5. $C(a) \to P(a)$ | UI from (4) |
> | 6. $P(a)$ | MP from (3) and (5) |
> | 7. $\neg B(a)$ | Simplification from (2) |
> | 8. $P(a) \land \neg B(a)$ | Conjunction from (6) and (7) |
> | 9. $\exists x(P(x) \land \neg B(x))$ | EG from (8) |
> 
> Key moves: Use EI to name the student who hasn't read the book. Use UI to apply the "everyone passed" rule to that specific student. Then recombine and generalize back with EG.

---

## Returning to Socrates

Now we can formally prove the Socrates argument:

$$\frac{\forall x(Man(x) \to Mortal(x)) \\ Man(Socrates)}{\therefore Mortal(Socrates)}$$

| Step | Reason |
|---|---|
| 1. $\forall x(Man(x) \to Mortal(x))$ | Premise |
| 2. $Man(Socrates) \to Mortal(Socrates)$ | UI from (1) |
| 3. $Man(Socrates)$ | Premise |
| 4. $Mortal(Socrates)$ | MP from (2) and (3) |

Just UI + Modus Ponens. This pattern is so common it gets its own name.

---

## Universal Modus Ponens

Combines universal instantiation and modus ponens into one step:

$$\frac{\forall x(P(x) \to Q(x)) \\ P(a)}{\therefore Q(a)}$$

where $a$ is a particular element in the domain.

Saves a step in proofs. Instead of explicitly doing UI then MP, you can just do UMP directly. This is what we really used in the Socrates example.
